fix some additional issues ignored in the last commit

viper-total-heaps/TotalSemantics.thy
@@ -365,27 +365,29 @@ definition vpr_method_correct_total_aux ::
           "'a total_context \<Rightarrow> ('a full_total_state \<Rightarrow> bool) \<Rightarrow> method_decl
                 \<Rightarrow> ('a total_context \<Rightarrow> ('a full_total_state \<Rightarrow> bool) \<Rightarrow> method_decl \<Rightarrow> 'a full_total_state \<Rightarrow> 'a full_total_state \<Rightarrow> bool)
                \<Rightarrow>  bool" where
-  "vpr_method_correct_total_aux ctxt R mdecl CorrectWrtPre \<equiv>
+  "vpr_method_correct_total_aux ctxt StateCons mdecl CorrectWrtPre \<equiv>
          (\<forall>(\<omega> :: 'a full_total_state) rpre.
             vpr_store_well_typed (absval_interp_total ctxt) (nth_option (method_decl.args mdecl @ method_decl.rets mdecl)) (get_store_total \<omega>) \<longrightarrow>
             total_heap_well_typed (program_total ctxt) (absval_interp_total ctxt) (get_hh_total_full \<omega>) \<longrightarrow>
             is_empty_total_full \<omega> \<longrightarrow>
-            red_inhale ctxt R (method_decl.pre mdecl) \<omega> rpre \<longrightarrow>
+            StateCons \<omega> \<longrightarrow>
+            red_inhale ctxt StateCons (method_decl.pre mdecl) \<omega> rpre \<longrightarrow>
             (
               rpre \<noteq> RFailure \<and>
               (\<forall>\<omega>pre. rpre = RNormal \<omega>pre \<longrightarrow>
-               CorrectWrtPre ctxt R mdecl \<omega>pre \<omega>
+               CorrectWrtPre ctxt StateCons mdecl \<omega>pre \<omega>
               )
             )
          )"
 
 lemma vpr_method_correct_total_aux_normalD:
-  assumes "vpr_method_correct_total_aux ctxt R mdecl CorrectWrtPre"
-      and "red_inhale ctxt R (method_decl.pre mdecl) \<omega> (RNormal \<omega>pre)"
+  assumes "vpr_method_correct_total_aux ctxt StateCons mdecl CorrectWrtPre"
+      and "red_inhale ctxt StateCons (method_decl.pre mdecl) \<omega> (RNormal \<omega>pre)"
       and "vpr_store_well_typed (absval_interp_total ctxt) (nth_option (method_decl.args mdecl @ method_decl.rets mdecl)) (get_store_total \<omega>)"
       and "total_heap_well_typed (program_total ctxt) (absval_interp_total ctxt) (get_hh_total_full \<omega>)"
       and "is_empty_total_full \<omega>"
-    shows "CorrectWrtPre ctxt R mdecl \<omega>pre \<omega>"
+      and "StateCons \<omega>"
+    shows "CorrectWrtPre ctxt StateCons mdecl \<omega>pre \<omega>"
   using assms
   unfolding vpr_method_correct_total_aux_def
   by blast
@@ -412,6 +414,7 @@ lemma vpr_postcondition_framed_assertion_framing_state:
       and "total_heap_well_typed (program_total ctxt) (absval_interp_total ctxt) (get_hh_total mh)"
       and "wf_mask_simple (get_mh_total mh)"
       and "trace old_label = Some \<phi>pre"
+      and "R \<omega>"
     shows "assertion_framing_state ctxt R postcondition \<omega>"
   using assms
   unfolding vpr_postcondition_framed_def
@@ -442,18 +445,19 @@ definition vpr_method_correct_total :: "'a total_context \<Rightarrow> ('a full_
        "
 
 definition vpr_method_correct_total_expanded :: "'a total_context \<Rightarrow> ('a full_total_state \<Rightarrow> bool) \<Rightarrow> method_decl \<Rightarrow> bool" where
-  "vpr_method_correct_total_expanded ctxt R mdecl \<equiv>
+  "vpr_method_correct_total_expanded ctxt StateCons mdecl \<equiv>
          (\<forall>(\<omega> :: 'a full_total_state) rpre.
             vpr_store_well_typed (absval_interp_total ctxt) (nth_option (method_decl.args mdecl @ method_decl.rets mdecl)) (get_store_total \<omega>) \<longrightarrow>
             total_heap_well_typed (program_total ctxt) (absval_interp_total ctxt) (get_hh_total_full \<omega>) \<longrightarrow>
             is_empty_total_full \<omega> \<longrightarrow>
-            red_inhale ctxt R (method_decl.pre mdecl) \<omega> rpre \<longrightarrow>
+            StateCons \<omega> \<longrightarrow>
+            red_inhale ctxt StateCons (method_decl.pre mdecl) \<omega> rpre \<longrightarrow>
             (
               rpre \<noteq> RFailure \<and>
               (\<forall>\<omega>pre. rpre = RNormal \<omega>pre \<longrightarrow>
                 \<comment>\<open>\<^term>\<open>get_store_total \<omega>\<close> should be equal to \<^term>\<open>get_store_total \<omega>pre\<close> since inhale does not change the store.\<close>
-                vpr_postcondition_framed ctxt R (method_decl.post mdecl) (get_total_full \<omega>pre) (get_store_total \<omega>) \<and>
-                (\<forall>mbody. method_decl.body mdecl = Some mbody \<longrightarrow> vpr_method_body_correct ctxt R mdecl \<omega>pre)
+                vpr_postcondition_framed ctxt StateCons (method_decl.post mdecl) (get_total_full \<omega>pre) (get_store_total \<omega>) \<and>
+                (\<forall>mbody. method_decl.body mdecl = Some mbody \<longrightarrow> vpr_method_body_correct ctxt StateCons mdecl \<omega>pre)
               )
             )
          )"
@@ -467,7 +471,7 @@ text \<open>\<^const>\<open>vpr_method_correct_total\<close> specifies when a Vi
       expanded version are equivalent.\<close>
 
 lemma vpr_method_correct_total_2_new_equiv:
-  "vpr_method_correct_total ctxt R mdecl = vpr_method_correct_total_expanded ctxt R mdecl"
+  "vpr_method_correct_total ctxt StateCons mdecl = vpr_method_correct_total_expanded ctxt StateCons mdecl"
   unfolding vpr_method_correct_total_def vpr_method_correct_total_expanded_def vpr_method_correct_total_aux_def
   by blast
 
